modified:   coq/test.v 	modified:   haskell/Set.hs 	new file:   haskell/book-info.hs 	modified:   haskell/category.hs 	new file:   haskell/error.hs 	new file:   haskell/object.hs 	modified:   haskell/test.hs 	new file:   haskell/time.hs 	modified:   polyglot/Composite/Composite.java 	modified:   polyglot/Composite/composite.c 	modified:   polyglot/Composite/composite.t.c 	new file:   scala/unicode.scala 	modified:   scm/evaluator/environment-test.scm 	modified:   scm/evaluator/environment2.scm 	modified:   scm/evaluator/frame.scm 	modified:   scm/evaluator/frame1.scm

haskell/Set.hs
@@ -33,10 +33,6 @@ instance (Eq a) => Ord (Set a) where
   (>=) x y = (subset y x)
   (<)  x y = (x <= y) && (x /= y)
   (>)  x y = (y <= x) && (x /= y) 
-   
 
-int :: Int -> Set Int
-int 0 = emptySet
-int n = union (singleton (n - 1)) (int (n - 1))
 
 
