haskell/category.hs
@@ -1,25 +1,37 @@
 import Set
 
-data Category arrow = Category { source   :: arrow -> arrow,
-                                 target   :: arrow -> arrow,
-                                 compose  :: arrow -> arrow -> arrow}
-
-
-
 -- underlying class (set in this case) of the category 
 -- of finite sets with elements of type a
-data Arrow a = Arrow (Set a) (Set a) (a -> a)
+class Categorizable a where
+  source :: a -> a
+  target :: a -> a
+  compose:: a -> a -> a
+ 
 
-setSource :: Arrow a -> Arrow a
-setSource (Arrow x y f) = Arrow x x (\u -> u)
+data FiniteSetArrow a = FSArrow (Set a) (Set a) (a -> a)
+instance (Eq a) => Categorizable (FiniteSetArrow a) where
+  source   (FSArrow x y f) = FSArrow x x (\u -> u)
+  target   (FSArrow x y f) = FSArrow y y (\u -> u)
+  compose  (FSArrow x y f) (FSArrow y' z g) = if (y == y') then 
+    FSArrow x z (g.f) else error "FSArrows are not composable"
 
-setTarget :: Arrow a -> Arrow a
-setTarget (Arrow x y f) = Arrow y y (\u -> u)
 
-setCompose :: (Eq a) => Arrow a -> Arrow a -> Arrow a
-setCompose (Arrow x y f) (Arrow y' z g) = if (y == y') then 
-  Arrow x z (\u ->  g (f u)) else error "Arrows are not composable"
+data PosetArrow a = PSArrow a a
+instance (Ord a) => Categorizable (PosetArrow a) where
+  source (PSArrow x y) = if x <= y then PSArrow x x else error "Illegal arrow"
+  target (PSArrow x y) = if x <= y then PSArrow y y else error "Illegal arrow"
+  compose(PSArrow x y) (PSArrow y' z) = 
+    if x <= y && y' <= z then
+      if y == y then
+        PSArrow x z
+      else
+        error "Poset arrows are not composable"
+    else
+      error "Illegal poset arrow arguments"
 
-finiteSet :: (Eq a) => Category (Arrow a)
-finiteSet = Category setSource setTarget setCompose
+
+
+
+
+
 
