haskell/object.hs
@@ -1,0 +1,4 @@
+class Member a where
+  method :: a -> b 
+
+
