scala/unicode.scala
@@ -1,0 +1,8 @@
+println("\u2200x(x\u2208y->y\u2208z)")
+println("arroa\bw")
+println(""" this is a multiline stri
+        ng which requires three '"' in a row""")
+
+// this screws up vim though....
+
+
