scm/evaluator/frame.scm
@@ -1,8 +1,10 @@
-(load "frame1")
 ; required interface for frame
 ;
 ; - insert! var val -> void
 ; - delete! var     -> void
 ; - find    var     -> (var,val) or #f
 ;
+
+; choose implementation here
+(load "frame1")
 (define frame frame1)
